rocq/path/Step2GeneratedClauses.v
@@ -9,13 +9,13 @@ Module Step2GeneratedClauses.
   Definition ClauseValid := @KairosOracleModel.ClauseValid.
   Definition origin := @KairosOracleModel.origin.
   Definition generated_item := @KairosOracleModel.generated_item.
+  Definition init_generated_items := @KairosOracleModel.init_generated_items.
   Definition ctx_matches_ps := @KairosOracleModel.ctx_matches_ps.
   Definition prod_clause := @KairosOracleModel.prod_obligation.
   Definition node_inv_clause := @KairosOracleModel.node_inv_obligation.
   Definition support_automaton_clause := @KairosOracleModel.support_automaton_obligation.
   Definition init_node_inv_clause := @KairosOracleModel.init_node_inv_obligation.
   Definition init_support_automaton_clause := @KairosOracleModel.init_support_automaton_obligation.
-  Definition gen_from_product_step := @KairosOracleModel.gen_from_product_step.
   Definition GeneratedBy := @KairosOracleModel.GeneratedBy.
   Definition Generated := @KairosOracleModel.Generated.
 End Step2GeneratedClauses.
